## [[Chain Rule Example]]
___

> [!quote] Chain Rule
> Suppose x is some function of t, then we know that:$$\dfrac{dx}{dt} = lim_{\triangle t \to 0} \dfrac{\triangle x}{\triangle t}$$
> Suppose that y is some function of x, then $$\dfrac{dy}{dx} = lim_{\triangle x \to 0} \dfrac{\triangle y}{\triangle x}$$
> We may also **consider y as a function of t, that is, y(x(t))** and calculate$$\dfrac{dy}{dt} = lim_{\triangle t \to 0} \dfrac{\triangle y}{\triangle t}$$
> How is $\dfrac{dy}{dt}$ related to $\dfrac{dy}{dx}$? We have the following rule:
> $$\dfrac{dy}{dt}= \dfrac{dy}{dx} \cdot \dfrac{dx}{dt}\quad - The\; Chain\; Rule$$
> *To remember this formula, think of the dx terms "cancelling"*

#calculus 