> [!quote] Proof of the Chain Rule
> **Consider a small change ($\triangle t$) in t.** 
> <br>
> **Then x(t) changes by** $\triangle x = x(t+\triangle t)$
> <br>
> **And y(x(t)) changes by**: $$\triangle y = y(x(t+\triangle t)) - y(x(t))$$
> $$ = y(x+\triangle x) - y(x)$$
> <br>
> **But**
> $$\dfrac{\triangle y}{\triangle t} = \dfrac{\triangle y}{\triangle x} \cdot \dfrac{\triangle x}{\triangle t} \quad (1)$$
> <br>
> *As $\triangle t \to 0, \triangle x \to 0$ and so $\dfrac{\triangle y}{\triangle x} \to \dfrac{dy}{dx}$ and $\dfrac{\triangle x}{\triangle t} \to \dfrac{dx}{dt}$ and the chain rule then follows from (1) upon letting $\triangle \to 0$*

#calculus 