>[!eq] 
>**Let:** 
>$a = a_1 \hat i + a_2 \hat j +a_3 \hat k$
>$b = b_1 \hat i + b_2 \hat j +b_3 \hat k$
>
>**Then:**
>$a\cdot b = a_1 b_1 + a_2 b_2 + a_3 b_3$
>
>**Or:**
>$$\sum_{i=1}^{n} ai\;bi = a\cdot b $$

___
## Proof:
$a\cdot \hat i = (a_1 \hat i + a_2 \hat j +a_3 \hat k) \cdot \hat i$
$a\cdot \hat i = (a_1 \hat i)\cdot\hat i + (a_2 \hat j)\cdot\hat i + (a_3 \hat k)\cdot\hat i \quad\quad \text{(distributive law)}$
$a\cdot \hat i = a_1 (\hat i\cdot\hat i) + a_2 (\hat j\cdot\hat i) + a_3 (\hat k\cdot\hat i) \quad\quad \text{(scalar multiplication)}$
$a\cdot \hat i = a_{1(1)}+ a2(0) + a3(0) \quad\quad\quad\quad\quad\; \text{(dot product rules)}$
$a\cdot \hat i = a_1$

Thus $a\cdot \hat i = a_1 \quad and \quad a\cdot \hat j = a_{2}\quad and\quad a\cdot\hat k = a_{3}$
Thus the components of $a$ can be recovered by taking scalar products with $\hat i, \hat j, \hat k$

Also:
$a\cdot b = a\cdot (b_{1}\hat i + b_{2}\hat j + b_{3}\hat k )$
$a\cdot b = (a\cdot \hat i)b_{1}+ (a\cdot \hat j)b_{2}+ (a\cdot \hat k)b_3$
$a\cdot b = a_{1}b_{1}+a_{2}b_{2}+ a_{3}b_{3}$
___
## More (short) proofs:
$a\cdot a = |a|^2$
$\quad\quad\, = a_{1}^{2}+a_{2}^2+a_{3}^2$

**and:**
$a = \sqrt{|a|^{2}}= \sqrt{a_{1}^{2}+a_{2}^2+a_{3}^2}$
